Style changes

Sequences/NatSeqConversions.dfy
@@ -29,17 +29,17 @@ abstract module NatSeqConversions refines NatSeq {
   }
 
   /* Converts a sequence from LargeBound.BOUND() to SmallBound.BOUND(). */
-  function method {:opaque} to_smaller_base(xs: seq<LargeBound.uint>): (ys: seq<SmallBound.uint>)
+  function method {:opaque} to_smaller_bound(xs: seq<LargeBound.uint>): (ys: seq<SmallBound.uint>)
     ensures |ys| == |xs| * E()
   {
     if |xs| == 0 then []
     else
       lemma_mul_is_distributive_add_other_way(E(), 1, |xs| - 1);
-      SmallBound.from_nat_with_len(first(xs), E()) + to_smaller_base(drop_first(xs))
+      SmallBound.from_nat_with_len(first(xs), E()) + to_smaller_bound(drop_first(xs))
   }
 
   /* Converts a sequence from SmallBound.BOUND() to LargeBound.BOUND(). */
-  function method {:opaque} to_larger_base(xs: seq<SmallBound.uint>): (ys: seq<LargeBound.uint>)
+  function method {:opaque} to_larger_bound(xs: seq<SmallBound.uint>): (ys: seq<LargeBound.uint>)
     requires |xs| % E() == 0
     ensures |ys| == |xs| / E()
   {
@@ -51,27 +51,27 @@ abstract module NatSeqConversions refines NatSeq {
       SmallBound.lemma_seq_nat_bound(xs[..E()]);
       lemma_mod_sub_multiples_vanish_auto();
       lemma_div_minus_one(|xs|, E());
-      [SmallBound.to_nat(xs[..E()]) as LargeBound.uint] + to_larger_base(xs[E()..])
+      [SmallBound.to_nat(xs[..E()]) as LargeBound.uint] + to_larger_bound(xs[E()..])
   }
 
   /* Sequence conversion from LargeBound.BOUND() to SmallBound.BOUND() does not
   change its nat representation. */
-  lemma lemma_smaller_base_to_nat(xs: seq<LargeBound.uint>)
-    ensures SmallBound.to_nat(to_smaller_base(xs)) == LargeBound.to_nat(xs)
+  lemma lemma_smaller_bound_to_nat(xs: seq<LargeBound.uint>)
+    ensures SmallBound.to_nat(to_smaller_bound(xs)) == LargeBound.to_nat(xs)
   {
     reveal LargeBound.to_nat();
     reveal SmallBound.to_nat();
-    reveal to_smaller_base();
+    reveal to_smaller_bound();
     if |xs| > 0 {
       calc {
-        SmallBound.to_nat(to_smaller_base(xs));
-        SmallBound.to_nat(SmallBound.from_nat_with_len(first(xs), E()) + to_smaller_base(drop_first(xs)));
-          { SmallBound.lemma_seq_prefix(SmallBound.from_nat_with_len(first(xs), E()) + to_smaller_base(drop_first(xs)), E()); }
-        SmallBound.to_nat(SmallBound.from_nat_with_len(first(xs), E())) + SmallBound.to_nat(to_smaller_base(drop_first(xs))) * power(SmallBound.BOUND(), E());
+        SmallBound.to_nat(to_smaller_bound(xs));
+        SmallBound.to_nat(SmallBound.from_nat_with_len(first(xs), E()) + to_smaller_bound(drop_first(xs)));
+          { SmallBound.lemma_seq_prefix(SmallBound.from_nat_with_len(first(xs), E()) + to_smaller_bound(drop_first(xs)), E()); }
+        SmallBound.to_nat(SmallBound.from_nat_with_len(first(xs), E())) + SmallBound.to_nat(to_smaller_bound(drop_first(xs))) * power(SmallBound.BOUND(), E());
           {
             SmallBound.lemma_from_nat_with_len_eq_from_nat(first(xs), E());
             SmallBound.lemma_nat_seq_nat(first(xs));
-            lemma_smaller_base_to_nat(drop_first(xs));
+            lemma_smaller_bound_to_nat(drop_first(xs));
           }
         first(xs) + LargeBound.to_nat(drop_first(xs)) * power(SmallBound.BOUND(), E());
           { assert power(SmallBound.BOUND(), E()) == LargeBound.BOUND(); }
@@ -82,23 +82,23 @@ abstract module NatSeqConversions refines NatSeq {
 
   /* Sequence conversion from SmallBound.BOUND() to LargeBound.BOUND() does not
   change its nat representation. */
-  lemma lemma_larger_base_to_nat(xs: seq<SmallBound.uint>)
+  lemma lemma_larger_bound_to_nat(xs: seq<SmallBound.uint>)
     requires |xs| % E() == 0
-    ensures LargeBound.to_nat(to_larger_base(xs)) == SmallBound.to_nat(xs)
+    ensures LargeBound.to_nat(to_larger_bound(xs)) == SmallBound.to_nat(xs)
   {
     reveal LargeBound.to_nat();
     reveal SmallBound.to_nat();
-    reveal to_larger_base();
+    reveal to_larger_bound();
     if |xs| > 0 {
       calc {
-        LargeBound.to_nat(to_larger_base(xs));
+        LargeBound.to_nat(to_larger_bound(xs));
           {
             lemma_mod_eq_zero(|xs|, E());
             lemma_mod_sub_multiples_vanish_auto();
             SmallBound.lemma_seq_nat_bound(xs[..E()]);
           }
-        LargeBound.to_nat([SmallBound.to_nat(xs[..E()]) as LargeBound.uint] + to_larger_base(xs[E()..]));
-          { lemma_larger_base_to_nat(xs[E()..]); }
+        LargeBound.to_nat([SmallBound.to_nat(xs[..E()]) as LargeBound.uint] + to_larger_bound(xs[E()..]));
+          { lemma_larger_bound_to_nat(xs[E()..]); }
         SmallBound.to_nat(xs[..E()]) + SmallBound.to_nat(xs[E()..]) * power(SmallBound.BOUND(), E());
           { SmallBound.lemma_seq_prefix(xs, E()); }
         SmallBound.to_nat(xs);
@@ -106,29 +106,29 @@ abstract module NatSeqConversions refines NatSeq {
     }
   }
 
-  /* to_smaller_base is injective. */
-  lemma lemma_to_smaller_base_is_injective(xs: seq<LargeBound.uint>,
-                                         ys: seq<LargeBound.uint>)
-    requires to_smaller_base(xs) == to_smaller_base(ys)
+  /* to_smaller_bound is injective. */
+  lemma lemma_to_smaller_bound_is_injective(xs: seq<LargeBound.uint>,
+                                            ys: seq<LargeBound.uint>)
+    requires to_smaller_bound(xs) == to_smaller_bound(ys)
     requires |xs| == |ys|
     ensures xs == ys
   {
-    lemma_smaller_base_to_nat(xs);
-    lemma_smaller_base_to_nat(ys);
+    lemma_smaller_bound_to_nat(xs);
+    lemma_smaller_bound_to_nat(ys);
     assert LargeBound.to_nat(xs) == LargeBound.to_nat(ys);
     LargeBound.lemma_seq_eq(xs, ys);
   }
 
-  /* to_larger_base is injective. */
-  lemma lemma_to_larger_base_is_injective(xs: seq<SmallBound.uint>,
-                                          ys: seq<SmallBound.uint>)
+  /* to_larger_bound is injective. */
+  lemma lemma_to_larger_bound_is_injective(xs: seq<SmallBound.uint>,
+                                           ys: seq<SmallBound.uint>)
     requires |xs| % E() == |ys| % E() == 0 
-    requires to_larger_base(xs) == to_larger_base(ys)
+    requires to_larger_bound(xs) == to_larger_bound(ys)
     requires |xs| == |ys|
     ensures xs == ys
   {
-    lemma_larger_base_to_nat(xs);
-    lemma_larger_base_to_nat(ys);
+    lemma_larger_bound_to_nat(xs);
+    lemma_larger_bound_to_nat(ys);
     assert SmallBound.to_nat(xs) == SmallBound.to_nat(ys);
     SmallBound.lemma_seq_eq(xs, ys);
   }
